Add base64 printing for testing

tests/Tests/HashString.lean
@@ -1,10 +1,8 @@
 import Blake3
+import BinaryTools
 
 open Blake3
 
-def String.toByteArray (s : String) : ByteArray :=
-  (List.map
-    (fun c : Char => c.toNat.toUInt8) s.toList).toByteArray
 
 /- HashString -/
 /- #eval Blake3.version -/
@@ -12,8 +10,10 @@ def String.toByteArray (s : String) : ByteArray :=
 
 def main (args : List String) : IO UInt32 := do
   try
-    IO.println Blake3.version
-    IO.println (hash "hello".toByteArray)
+    IO.println s!"Blake3 version: {Blake3.version}"
+    let tests := #["hello", "More complicated test"]
+    for s in tests do
+      IO.println s!"blake3('{s}')={(Blake3.hash s.toByteArray)}"
     pure 0
   catch e =>
     IO.eprintln <| "error: " ++ toString e -- avoid "uncaught exception: ..."
