src/BinaryTools.lean
@@ -1,0 +1,105 @@
+/-
+BinaryTools: Utilities for displaying and manipulating Binary data.
+-/
+
+/-
+Simplification rules for ensuring type safety of Blake3Hash
+-/
+@[simp] theorem ByteArray.size_empty : ByteArray.empty.size = 0 :=
+rfl
+
+@[simp] theorem ByteArray.size_push (B : ByteArray) (a : UInt8) : (B.push a).size = B.size + 1 :=
+by { cases B; simp only [ByteArray.push, ByteArray.size, Array.size_push] }
+
+@[simp] theorem List.to_ByteArray_size : (L : List UInt8) → L.toByteArray.size = L.length
+| [] => rfl
+| a::l => by simp [List.toByteArray, to_ByteArray_loop_size]
+where to_ByteArray_loop_size :
+  (L : List UInt8) → (B : ByteArray) → (List.toByteArray.loop L B).size = L.length + B.size
+| [], B => by simp [List.toByteArray.loop]
+| a::l, B => by
+    simp [List.toByteArray.loop, to_ByteArray_loop_size]
+    rw [Nat.add_succ, Nat.succ_add]
+
+universe u
+universe v
+
+/-
+Type class for default conversion between two types.
+-/
+class Into (Target: Type v) (Source: Type u) :=
+  (into: Source → Target)
+
+export Into (into)
+
+instance (A: Type u) : Into A A := ⟨id⟩
+
+def String.toByteArray (s : String) : ByteArray :=
+  (List.map
+    (fun c : Char => c.toNat.toUInt8) s.toList).toByteArray
+
+instance : Into ByteArray String := {
+  into := String.toByteArray
+}
+
+namespace Alphabet
+def base2: String := "01"
+def base8: String := "01234567"
+def base10: String := "0123456789"
+def base16: String := "0123456789abcdef"
+def base16upper: String := "0123456789ABCDEF"
+def base32: String := "abcdefghijklmnopqrstuvwxyz234567"
+def base32upper: String := "ABCDEFGHIJKLMNOPQRSTUVWXYZ234567"
+def base32hex : String := "0123456789abcdefghijklmnopqrstuv"
+def base32hexupper : String := "0123456789ABCDEFGHIJKLMNOPQRSTUV"
+def base32z : String := "ybndrfg8ejkmcpqxot1uwisza345h769"
+def base36 : String := "0123456789abcdefghijklmnopqrstuvwxyz"
+def base36upper : String := "0123456789ABCDEFGHIJKLMNOPQRSTUVWXYZ"
+def base58flickr : String := 
+  "123456789abcdefghijkmnopqrstuvwxyzABCDEFGHJKLMNPQRSTUVWXYZ"
+def base58btc : String := 
+  "123456789ABCDEFGHJKLMNPQRSTUVWXYZabcdefghijkmnopqrstuvwxyz"
+def base64 : String := 
+  "ABCDEFGHIJKLMNOPQRSTUVWXYZabcdefghijklmnopqrstuvwxyz0123456789+/"
+def base64url : String := 
+  "ABCDEFGHIJKLMNOPQRSTUVWXYZabcdefghijklmnopqrstuvwxyz0123456789-_"
+
+end Alphabet
+
+/-
+Encode a ByteArray as a base64 String
+-/
+def toBase64 {I: Type u} [Into ByteArray I] (input : I) (pad: Bool := true) : String := do
+  let input : ByteArray := Into.into input
+  let x := ByteArray.size input % 3
+  let mut bytes := input
+  let mut str := ""
+  if x == 1 then bytes := bytes.append [0x00, 0x00].toByteArray
+  if x == 2 then bytes := bytes.append [0x00].toByteArray
+  for i in [:(bytes.size / 3)] do
+    let b0 := bytes.data[3 * i]
+    let b1 := bytes.data[3 * i + 1]
+    let b2 := bytes.data[3 * i + 2]
+    let s0 := b0.shiftRight 2
+    let s1 := UInt8.xor
+      ((b0.land 0b00000011).shiftLeft 4) 
+      ((b1.land 0b11110000).shiftRight 4)
+    let s2 := UInt8.xor
+      ((b1.land 0b00001111).shiftLeft 2) 
+      ((b2.land 0b11000000).shiftRight 6)
+    let s3 := b2.land 0b00111111
+    str := str.push (Alphabet.base64.get s0.toNat)
+    str := str.push (Alphabet.base64.get s1.toNat)
+    str := str.push (Alphabet.base64.get s2.toNat)
+    str := str.push (Alphabet.base64.get s3.toNat)
+  if pad then do
+    if x == 1 then 
+      str := str.set (str.length - 1) '='
+      str := str.set (str.length - 2) '='
+    if x == 2 then 
+      str := str.set (str.length - 1) '='
+    return str
+  else 
+    if x == 1 then str := str.dropRight 2
+    if x == 2 then str := str.dropRight 1
+    return str
