src/Blake3.lean
@@ -1,6 +1,8 @@
 /-
- Bindings to the Blake3 hashing library.
+Bindings to the Blake3 hashing library.
 -/
+import BinaryTools
+
 namespace Blake3
 
 /-
@@ -13,46 +15,27 @@ constant BLAKE3_CHUNK_LEN: Nat := 1024
 constant BLAKE3_MAX_DEPTH: Nat := 54
 
 /-
-Simplification rules for ensuring type safety of Blake3Hash
--/
-@[simp] theorem ByteArray.size_empty : ByteArray.empty.size = 0 :=
-rfl
-
-@[simp] theorem ByteArray.size_push (B : ByteArray) (a : UInt8) : (B.push a).size = B.size + 1 :=
-by { cases B; simp only [ByteArray.push, ByteArray.size, Array.size_push] }
-
-@[simp] theorem List.to_ByteArray_size : (L : List UInt8) → L.toByteArray.size = L.length
-| [] => rfl
-| a::l => by simp [List.toByteArray, to_ByteArray_loop_size]
-where to_ByteArray_loop_size :
-  (L : List UInt8) → (B : ByteArray) → (List.toByteArray.loop L B).size = L.length + B.size
-| [], B => by simp [List.toByteArray.loop]
-| a::l, B => by
-    simp [List.toByteArray.loop, to_ByteArray_loop_size]
-    rw [Nat.add_succ, Nat.succ_add]
-/-
 A dependent ByteArray which guarantees the correct byte length.
 -/
 def Blake3Hash : Type := { r : ByteArray // r.size = BLAKE3_OUT_LEN }
 
-deriving instance ToString for Blake3Hash
+@[defaultInstance]
+instance : Into ByteArray Blake3Hash := ⟨Subtype.val⟩
+
+instance : Into String Blake3Hash := ⟨toBase64⟩
+
+instance : ToString Blake3Hash := ⟨into⟩
 
 instance : Inhabited Blake3Hash where
   default := ⟨(List.replicate BLAKE3_OUT_LEN 0).toByteArray, by simp⟩
 
 
-/- @[extern "lean_blake3_initialize"] -/
 constant HasherPointed : PointedType
+
 def Hasher : Type := HasherPointed.type
+
 instance : Inhabited Hasher := ⟨HasherPointed.val⟩
 
-/-
-Perform an unsafe IO operation for use in a pure context.
--/
-unsafe def unsafeIO' [Inhabited α] (k : IO α) : α :=
-  match unsafeIO k with
-  | Except.ok a => a
-  | Except.error e => panic e.toString
 
 /-
 Version of the linked BLAKE3 implementation library.
@@ -69,21 +52,20 @@ Initialize a hasher.
 constant initHasher : Unit → Hasher
 
 
-/- @[extern "blake3_hasher_init_keyed"] -/
-/- constant initHasherKeyed (key: Array UInt8) : Hasher -/
+@[extern "blake3_hasher_init_keyed"]
+constant initHasherKeyed (key: Array UInt8) : Hasher
 
 
-/- @[extern "blake3_hasher_init_derive_key"] -/
-/- constant initHasherDeriveKey (context: String) : Hasher -/
+@[extern "blake3_hasher_init_derive_key"]
+constant initHasherDeriveKey (context: String) : Hasher
 
-/- @[extern "blake3_hasher_init_derive_key_raw"] -/
-/- constant initHasherDeriveKeyRaw (context: String) (contextLength : USize) : Hasher -/
+@[extern "blake3_hasher_init_derive_key_raw"]
+constant initHasherDeriveKeyRaw (context: String) (contextLength : USize) : Hasher
 
 
 /-
 Put more data into the hasher. This can be called several times.
 -/
-/- @[implementedBy hasherUpdateImpl] -/
 @[extern "lean_blake3_hasher_update"]
 constant hasherUpdate (hasher : Hasher) (input : ByteArray) (length : USize) : Hasher
 
@@ -96,8 +78,8 @@ constant hasherFinalize : (hasher : Hasher) → (length : USize) → ByteArray
 /-
 Finalize the hasher and write the output to an initialized array.
 -/
-/- @[extern "blake3_hasher_finalize_seek"] -/
-/- constant hasherFinalizeSeek : (hasher : Hasher) → (seek : UInt64) → (length : USize) → ByteArray -/
+@[extern "blake3_hasher_finalize_seek"]
+constant hasherFinalizeSeek : (hasher : Hasher) → (seek : UInt64) → (length : USize) → ByteArray
 
 /-
 Hash a ByteArray
